all_mach.v
@@ -1,2 +1,2 @@
 Require Export all_cont.
-Require Export core.mach.exec core.mach.Mmach.
+Require Export FMop Umach Ucont Uuniv.
