core/mach/Duop.v
@@ -1,0 +1,46 @@
+From mathcomp Require Import ssreflect seq ssrnat ssrbool eqtype ssrfun.
+From rlzrs Require Import all_mf.
+Require Import all_cont FMop Umach Ucont Uuniv.
+
+Set Implicit Arguments.
+Unset Strict Implicit.
+Unset Printing Implicit Defensive.
+
+Section duality_operator.
+(* Q: Questions, A: Answers *)
+Context (Q Q' A A' : Type).
+(* B: Baire space *)
+Notation B := (Q -> A).
+Notation B' := (Q' -> A').
+Notation "? K" := (@inl (list Q) A' K) (format "'?' K", at level 50).
+Notation "! a'" := (@inr (list Q) A' a') (format "'!' a'", at level 50).
+
+Fixpoint collect_left (Ka's: seq (seq Q + A')) : seq Q :=
+  match Ka's with
+  | nil => nil
+  | cons Ka' Ka's' => match Ka' with
+                      | inl K => K ++ collect_left Ka's'
+                      | inr a' => nil
+                      end
+  end.
+
+                                             
+Fixpoint D (phi: B) (Ka'sq': seq (seq Q + A') * Q') : seq (seq A * Q') + A' :=
+  match Ka'sq'.1 with
+    | nil => inl [::(nil, Ka'sq'.2)]
+    | Ka' :: Ka's => match Ka' with
+                    | inl K => inl [::(map phi (collect_left Ka'sq'.1), Ka'sq'.2)]
+                    | inr a' => inr a'
+                    end
+  end.
+
+Lemma D_spec psi phi:
+  \F_(U (D phi)) psi === \F_(U psi) phi.
+Proof.
+move => Fphi.
+split => /FU_spec evl q'; last first.
+have [Qn com]:= evl q'.
+exists (size Qn).+2.
+elim: Qn com => [[_ /= val] | K Qn ih com]; first by rewrite /= /U /= /U_step/= val.
+Admitted.
+End duality_operator.
